test/arrayptrs.c
@@ -13,13 +13,13 @@ void write_via_ptr(_array int *a)
 
 _include_pulse(
   let unless_null #a (x: array a) (p: slprop) : slprop =
-    if Pulse.Lib.Array.is_null x then emp else p
+    if array_is_null x then emp else p
 
   [@@pulse_intro]
   ghost fn intro_unless_null_null (#a: Type0) p
-    ensures unless_null #a Pulse.Lib.Array.null p
+    ensures unless_null #a array_null p
   {
-    rewrite emp as unless_null #a Pulse.Lib.Array.null p
+    rewrite emp as unless_null #a array_null p
   }
 
   [@@pulse_intro]
@@ -27,9 +27,9 @@ _include_pulse(
     requires p
     ensures unless_null x p
   {
-    if Pulse.Lib.Array.is_null x {
+    if array_is_null x {
       drop_ p;
-      assert rewrites_to x Pulse.Lib.Array.null;
+      assert rewrites_to x array_null;
     } else {
       rewrite p as unless_null x p;
     }
@@ -37,13 +37,13 @@ _include_pulse(
 
   ghost fn elim_unless_null_null (#a: Type0) (x: array a) p
     requires unless_null x p
-    requires pure (Pulse.Lib.Array.is_null x)
+    requires pure (array_is_null x)
   {
     rewrite unless_null x p as emp
   }
   ghost fn elim_unless_null_nonnull (#a: Type0) (x: array a) p
     requires unless_null x p
-    requires pure (not (Pulse.Lib.Array.is_null x))
+    requires pure (not (array_is_null x))
     ensures p
   {
     rewrite unless_null x p as p
@@ -51,22 +51,24 @@ _include_pulse(
 )
 
 _include_pulse(
-  let is_slice_prop #a (lo hi: array a) (x: array a) (v: Seq.seq (option a)) (m: nat->prop) =
-    offset_of x <= offset_of lo
+  unfold
+  let is_slice_prop #a (lo hi: array a) (x: array a) (v: full_array_spec a) =
+    base_of lo == base_of x /\ base_of hi == base_of x
+      /\ offset_of x <= offset_of lo
       /\ offset_of lo <= offset_of hi
-      /\ offset_of hi <= offset_of x + Seq.length v
-      /\ (forall i. offset_of lo <= i /\ i < offset_of hi ==>
-        (m (i - offset_of x) /\ Some? (Seq.index v (i - offset_of x))))
+      /\ offset_of hi <= offset_of x + array_spec_len v
+      /\ (forall (i: nat). offset_of lo <= i /\ i < offset_of hi ==>
+        (array_spec_mask v (i - offset_of x) /\ array_spec_initd v (i - offset_of x)))
 
   [@@pulse_eager_unfold]
-  let is_slice #a (lo hi: array a) (x: array a) p v m =
-    pts_to_mask x #p v m ** 
+  let is_slice #a (lo hi: array a) (x: array a) p (v: full_array_spec a) =
+    array_pts_to x p v **
     arrayptr_pts_to lo x ** arrayptr_pts_to hi x **
-    pure (is_slice_prop lo hi x v m)
+    pure (is_slice_prop lo hi x v)
 )
 
-_arrayptr int *binary_search(_arrayptr int *lo, _arrayptr int *hi, int target)
-  _preserves(_inline_pulse(is_slice $(lo) $(hi) $`arr $`p_arr $`v_arr $`m_arr))
+_arrayptr const int *binary_search(_arrayptr const int *lo, _arrayptr const int *hi, int target)
+  _preserves(_inline_pulse(is_slice $(lo) $(hi) $`arr $`p_arr $`v_arr))
   _requires((bool) _inline_pulse(offset_of $(hi) - offset_of $(lo) < 100000))
   _ensures(_inline_pulse(unless_null $(return)
     (arrayptr_pts_to $(return) (arrayptr_parent $(lo)) **
@@ -77,10 +79,10 @@ _arrayptr int *binary_search(_arrayptr int *lo, _arrayptr int *hi, int target)
     _invariant(_live(hi))
     _invariant(_inline_pulse(arrayptr_pts_to $(lo) (old <| arrayptr_parent $(lo))))
     _invariant(_inline_pulse(arrayptr_pts_to $(hi) (old <| arrayptr_parent $(hi))))
-    _invariant((bool) _inline_pulse(offset_of $(lo) <= offset_of $(hi)))
+    _invariant((bool) _inline_pulse(is_slice_prop $(lo) $(hi) $`arr $`v_arr))
     _invariant((bool) _inline_pulse(old (offset_of $(lo)) <= offset_of $(lo) && offset_of $(hi) <= old (offset_of $(hi))))
   {
-      int *mid = lo + (hi - lo) / 2;
+      const int *mid = lo + (hi - lo) / 2;
       if (*mid == target)
         return mid;
       else if (*mid < target)
@@ -91,12 +93,12 @@ _arrayptr int *binary_search(_arrayptr int *lo, _arrayptr int *hi, int target)
   return NULL;
 }
 
-void use_binary_search(_array int *arr, int target, size_t length)
+void use_binary_search(_array const int *arr, int target, size_t length)
   _requires(length == arr._length && length <= 10000)
 {
-  _arrayptr int *lo = arr;
-  _arrayptr int *hi = arr + length;
-  _arrayptr int *result = binary_search(lo, hi, target);
+  _arrayptr const int *lo = arr;
+  _arrayptr const int *hi = arr + length;
+  _arrayptr const int *result = binary_search(lo, hi, target);
   if (result == NULL) {
     _ghost_stmt(elim_unless_null_null _ _);
   } else {
